\begin{table}
    \centering
    \begin{tabular}{|c|cc|}
    \hline
    A & 
    {
      $\begin{aligned}
        A(0, \lnot (\phi \lor \psi)) =&\ \lnot \phi\\ 
        A(0, \phi \land \psi) =&\ \phi\\ 
        A(0, \lnot (\phi \to \psi)) =&\ \phi\\ 
        A(0, \phi \liff \psi) =&\ \phi \limp \psi
      \end{aligned}$
    } &  
    {
      $\begin{aligned}
        A(1, \lnot (\phi \lor \psi)) =&\ \lnot \psi\\
        A(1, \phi \land \psi) =&\  \psi\\
        A(1, \lnot (\phi \to \psi)) =&\  \lnot \psi\\
        A(1, \phi \liff \psi) =&\  \psi \limp \phi
      \end{aligned}$
    } 
    \\ \hline
    B &
    {
      $\begin{aligned}
        B(0, \phi \lor \psi) =&\  \phi\\ 
        B(0, \lnot (\phi \land \psi)) =&\  \lnot \phi\\ 
        B(0, \phi \to \psi) =&\  \lnot \phi\\ 
        B(0, \lnot (\phi \liff \psi)) =&\  \lnot \phi \limp \psi
      \end{aligned}$
    } &  
    {
      $\begin{aligned}
        B(1, \phi \lor \psi) =&\  \psi\\
        B(1, \lnot (\phi \land \psi)) =&\  \lnot \psi\\
        B(1, \phi \to \psi) =&\  \psi\\
        B(1, \lnot (\phi \liff \psi)) =&\  \lnot \psi \limp \phi
      \end{aligned}$
    } 
    \\ \hline
    C & 
    $C(t, \forall \phi) = \phi [0 \mapsto t]$ &
    $C(t, \lnot \exists \phi) = \lnot \phi [0 \mapsto t]$
     \\ \hline
    D & 
    $D(k, \exists \phi) = \phi [0 \mapsto \idf{k}(\cdot)]$) &
    $D(k, \lnot \forall \phi) = \lnot \phi [0 \mapsto \idf{k}(\cdot)]$ 
    \\ \hline
    \end{tabular}
      \caption{
        Formula analysis functions. For any arguments not explicitly defined above, 
        the functions all return $\top$. E.g., $A(0, \phi \lor \psi) = \top$.
      }
      \label{tab:faf}
    \end{table}
    